pcuic/theories/PCUICInst.v
@@ -2183,7 +2183,7 @@ Proof.
           { eapply well_subst_app_up => //. }
           rewrite /brctxty /= case_branch_context_length //.
     * rewrite /predctx case_predicate_context_length //.
-  - intros Σ wfΣ Γ wfΓ p c u mdecl idecl pdecl isdecl args X X0 hc ihc e ty
+  - intros Σ wfΣ Γ wfΓ p c u mdecl idecl cdecl pdecl isdecl args X X0 hc ihc e ty
            Δ σ hΔ hσ.
     simpl.
     eapply meta_conv; [econstructor|].
