template-coq/theories/Typing.v
@@ -827,7 +827,7 @@ Inductive typing `{checker_flags} (Σ : global_env_ext) (Γ : context) : term ->
     Σ ;;; Γ |- tCase ci p c brs : mkApps ptm (indices ++ [c])
 
 | type_Proj p c u :
-    forall mdecl idecl pdecl (isdecl : declared_projection Σ.1 p mdecl idecl pdecl) args,
+    forall mdecl idecl cdecl pdecl (isdecl : declared_projection Σ.1 p mdecl idecl cdecl pdecl) args,
     Σ ;;; Γ |- c : mkApps (tInd (fst (fst p)) u) args ->
     #|args| = ind_npars mdecl ->
     Σ ;;; Γ |- tProj p c : subst0 (c :: List.rev args) (subst_instance u pdecl.2)
@@ -1187,7 +1187,7 @@ Lemma typing_ind_env `{cf : checker_flags} :
         P Σ Γ (tCase ci p c brs) (mkApps ptm (indices ++ [c]))) ->
 
     (forall Σ (wfΣ : wf Σ.1) (Γ : context) (wfΓ : wf_local Σ Γ) (p : projection) (c : term) u
-          mdecl idecl pdecl (isdecl : declared_projection Σ.1 p mdecl idecl pdecl) args,
+          mdecl idecl cdecl pdecl (isdecl : declared_projection Σ.1 p mdecl idecl cdecl pdecl) args,
         Forall_decls_typing P Σ.1 -> 
         PΓ Σ Γ wfΓ ->
         Σ ;;; Γ |- c : mkApps (tInd (fst (fst p)) u) args ->
